adding correct_proof of eval_ins/eval_ins_len

proof/CorrectRel.v
@@ -138,6 +138,10 @@ Definition MyListType_correct (b:block) (len: nat) (l: MyListType) (v: val) (stm
 Definition pc_correct (x: nat) (v: val) (st: State.state) (m:Memory.Mem.mem) :=
   Vint (Int.repr (Z.of_nat x)) = v /\  0 <= Z.of_nat x < Z.of_nat (mrs_num st) /\ 0 <= 8 * Z.of_nat (mrs_num st) <= Ptrofs.max_unsigned. (**r the number of input instructions should be less than Ptrofs.max_unsigned *)
 
+Definition ins_idx_correct (x: int) (v: val) (st: State.state) (m:Memory.Mem.mem) :=
+  Vint x = v /\
+  0 <= Int.signed x < Z.of_nat (ins_len st).
+
 
 Definition len_correct (len: nat) (x: int) (v: val) :=
   Vint x = v /\  Int.signed x = Z.of_nat len.
