simulation/correct_eval_ins.v
@@ -1,0 +1,113 @@
+From bpf.comm Require Import State Monad.
+From Coq Require Import List Lia ZArith.
+From compcert Require Import Integers Values Clight Memory.
+Import ListNotations.
+
+From bpf.proof Require Import Clightlogic MatchState CorrectRel CommonLemma.
+
+From bpf.clight Require Import interpreter.
+
+
+(**
+Check eval_ins.
+eval_ins
+     : int -> M int64
+*)
+
+Section Eval_ins.
+
+  (** The program contains our function of interest [fn] *)
+  Definition p : Clight.program := prog.
+
+  (* [Args,Res] provides the mapping between the Coq and the C types *)
+  (* Definition Args : list CompilableType := [stateCompilableType].*)
+  Definition args : list Type := [(int:Type)].
+  Definition res : Type := (int64:Type).
+
+  (* [f] is a Coq Monadic function with the right type *)
+  Definition f : arrow_type args (M res) := eval_ins.
+
+  Variable state_block: block. (**r a block storing all rbpf state information? *)
+  Variable mrs_block: block.
+  Variable ins_block: block.
+
+  (* [fn] is the Cligth function which has the same behaviour as [f] *)
+  Definition fn: Clight.function := f_eval_ins.
+
+  Definition stateM_correct (st:unit) (v: val) (stm:State.state) (m: Memory.Mem.mem) :=
+    v = Vptr state_block Ptrofs.zero /\ match_state state_block mrs_block ins_block stm m.
+
+  (* [match_arg] relates the Coq arguments and the C arguments *)
+  Definition match_arg_list : DList.t (fun x => x -> val -> State.state -> Memory.Mem.mem -> Prop) ((unit:Type) ::args) :=
+    DList.DCons stateM_correct
+      (DList.DCons ins_idx_correct
+        (DList.DNil _)).
+
+  (* [match_res] relates the Coq result and the C result *)
+  Definition match_res : res -> val -> State.state -> Memory.Mem.mem -> Prop := fun x v st m => int64_correct x v.
+
+  Instance correct_function3_eval_ins : forall a, correct_function3 p args res f fn nil false match_arg_list match_res a.
+  Proof.
+    correct_function_from_body args.
+    correct_body.
+    repeat intro.
+    unfold INV in H.
+    get_invariant _st.
+    get_invariant _idx.
+    unfold stateM_correct in c0.
+    destruct c0 as (Hv_eq & Hst).
+    unfold ins_idx_correct in c1.
+    destruct c1 as (Hc_eq & Hc_range).
+    (**r I should say idx is less than Int.max_signed *)
+    subst.
+
+    (** we need to get the value of pc in the memory *)
+    destruct Hst. clear - p0 p1 Hc_range mins_len mins.
+    destruct mins_len as (Hload_eq & Hge).
+    destruct mins as (Hins_eq & Hlen & Hle & Hmatch).
+    eexists; exists m, Events.E0.
+
+    split.
+    {
+      forward_star.
+      unfold Coqlib.align; rewrite Ptrofs.add_zero_l.
+      simpl.
+      unfold Mem.loadv in Hins_eq.
+      apply Hins_eq.
+      reflexivity.
+      fold Ptrofs.zero; rewrite Ptrofs.add_zero_l.
+      simpl.
+      unfold match_list_ins in Hmatch.
+      unfold Ptrofs.mul.
+      unfold Ptrofs.of_ints.
+      change (Ptrofs.unsigned (Ptrofs.repr 8)) with 8%Z.
+      rewrite Ptrofs.unsigned_repr with (z:= (Int.signed c)); [| lia].
+      rewrite Ptrofs.unsigned_repr; [| lia].
+      rewrite Hlen in Hmatch.
+      assert (Hnat: (0 <= Z.to_nat (Int.signed c) < ins_len st)%nat). {
+        lia.
+      }
+      specialize (Hmatch _ Hnat); clear Hnat.
+      unfold Mem.loadv in Hmatch.
+      assert (Hnat: Z.of_nat (Z.to_nat (Int.signed c)) = Int.signed c). { apply Z2Nat.id. lia. }
+      rewrite Hnat in Hmatch; clear Hnat.
+      rewrite Ptrofs.unsigned_repr in Hmatch; [| lia].
+      apply Hmatch.
+      reflexivity.
+      forward_star.
+    }
+    split.
+    {
+      unfold match_res, State.eval_ins, int64_correct, List64.MyListIndexs32, List64.MyList.index_s32.
+      reflexivity.
+    }
+    split.
+    {
+      constructor.
+    }
+    split; reflexivity.
+  Qed.
+
+End Eval_ins.
+
+Existing  Instance correct_function3_eval_ins.
