simulation/correct_eval_ins_len.v
@@ -1,0 +1,91 @@
+From bpf.comm Require Import State Monad.
+From Coq Require Import List Lia ZArith.
+From compcert Require Import Integers Values Clight Memory.
+Import ListNotations.
+
+From bpf.proof Require Import Clightlogic MatchState CorrectRel CommonLemma.
+
+From bpf.clight Require Import interpreter.
+
+
+(**
+Check eval_ins_len.
+eval_ins_len
+     : M int
+*)
+
+Section Eval_ins_len.
+
+  (** The program contains our function of interest [fn] *)
+  Definition p : Clight.program := prog.
+
+  (* [Args,Res] provides the mapping between the Coq and the C types *)
+  (* Definition Args : list CompilableType := [stateCompilableType].*)
+  Definition args : list Type := [].
+  Definition res : Type := (int:Type).
+
+  (* [f] is a Coq Monadic function with the right type *)
+  Definition f : arrow_type args (M res) := eval_ins_len.
+
+  Variable state_block: block. (**r a block storing all rbpf state information? *)
+  Variable mrs_block: block.
+  Variable ins_block: block.
+
+  (* [fn] is the Cligth function which has the same behaviour as [f] *)
+  Definition fn: Clight.function := f_eval_ins_len.
+
+  Definition stateM_correct (st:unit) (v: val) (stm:State.state) (m: Memory.Mem.mem) :=
+    v = Vptr state_block Ptrofs.zero /\ match_state state_block mrs_block ins_block stm m.
+
+  (* [match_arg] relates the Coq arguments and the C arguments *)
+  Definition match_arg_list : DList.t (fun x => x -> val -> State.state -> Memory.Mem.mem -> Prop) ((unit:Type) ::args) :=
+    DList.DCons stateM_correct (DList.DNil _).
+
+  (* [match_res] relates the Coq result and the C result *)
+  Definition match_res : res -> val -> State.state -> Memory.Mem.mem -> Prop := fun x v st m => x = Int.repr (Z.of_nat (ins_len st)).
+
+  Instance correct_function3_eval_ins_len : forall a, correct_function3 p args res f fn nil false match_arg_list match_res a.
+  Proof.
+    correct_function_from_body args.
+    correct_body.
+    repeat intro.
+    unfold INV in H.
+    get_invariant _st.
+    unfold stateM_correct in c.
+    destruct c as (Hv_eq & Hst).
+    subst.
+
+    (** we need to get the value of pc in the memory *)
+    destruct Hst. clear - p0 mins_len.
+    destruct mins_len as (Hload_eq & Hge).
+
+    eexists; exists m, Events.E0.
+
+    split.
+    {
+      forward_star.
+      unfold Coqlib.align; rewrite Ptrofs.add_zero_l.
+      unfold Ptrofs.zero; simpl.
+      unfold Mem.loadv in Hload_eq.
+      apply Hload_eq.
+      simpl.
+      reflexivity.
+      forward_star.
+    }
+    split.
+    {
+      unfold match_res, State.eval_ins_len.
+      reflexivity.
+    }
+    split.
+    {
+      constructor.
+      reflexivity.
+    }
+    simpl.
+    split; reflexivity.
+  Qed.
+
+End Eval_ins_len.
+
+Existing  Instance correct_function3_eval_ins_len.
